#254 exemplary definition

abp/generated/abp/FairMediumAutomaton.thy
@@ -6,7 +6,7 @@
  * Generated on Oct 12, 2018 5:31:31 PM by isartransformer 2.0.0
  *)
 theory FairMediumAutomaton
-  imports MediumDatatype FairMediumStates automat.ndAutomaton
+  imports MediumDatatype FairMediumStates automat.ndAutomaton automat.ndaComplete automat.ndaTotal
 
 begin
 
@@ -35,13 +35,20 @@ definition fairMediumTransition :: "(FairMediumState \<times> ('e::countable) me
 "fairMediumTransition = (\<lambda> (s,b). (if (sbeDom b) = mediumDom then fairMediumTransitionH (s, (mediumElem_get_i b)) else undefined))"
 
 (* Initial states with initial outputs *)
+(* SWS: Why setflat? *)
 definition fairMediumInitials :: "(FairMediumState \<times> ('e::countable) mediumMessage tsyn SB) set rev" where
-"fairMediumInitials = Rev (setflat\<cdot>{{(FairMediumState Single (var_counter::nat), (mediumOut_o null)) | var_counter . (var_counter>=0)}})"
+"fairMediumInitials = Rev ({(FairMediumState Single (var_counter::nat), (mediumOut_o null)) | var_counter . (var_counter>=0)})"
 
 (* The final automaton *)
-lift_definition fairMediumAutomaton :: "(FairMediumState, ('e::countable) mediumMessage tsyn) ndAutomaton" is
+lift_definition fairMediumAutomaton_incomplete :: "(FairMediumState, ('e::countable) mediumMessage tsyn) ndAutomaton" is
 "(fairMediumTransition, fairMediumInitials, Discr mediumDom, Discr mediumRan)"
   by (simp add: mediumDom_def mediumRan_def)
+
+(* SWS: Erstmal nur completion-chaos. Der rest läuft noch nicht. 
+   Soll aber so ähnlich aussehen, die function heißt dann "ndaErrorCompletion" *)
+definition fairMediumAutomaton :: "(FairMediumState, ('e::countable) mediumMessage tsyn) ndAutomaton" where
+"fairMediumAutomaton = ndaChaosCompletion fairMediumAutomaton_incomplete"
+                             
 
 (* Stream processing function for each state (handy for step lemmata) *)
 definition fairMediumStep :: "FairMediumState \<Rightarrow> ('e::countable) mediumMessage tsyn SPS" where
@@ -54,30 +61,44 @@ definition fairMediumSPS :: "('e::countable) mediumMessage tsyn SPS" where
 
 section \<open>Lemmas for automaton definition\<close>
 
-lemma fairmediumautomaton_trans[simp]: "ndaTransition\<cdot>fairMediumAutomaton = fairMediumTransition"
-  by(simp add: fairMediumAutomaton.rep_eq ndaTransition.rep_eq)
+lemma fairmediumautomaton_trans[simp]: "ndaTransition\<cdot>fairMediumAutomaton = chaosTransCompletion fairMediumTransition"
+  apply(simp add: fairMediumAutomaton_def)
+  by(simp add: ndaTransition.rep_eq fairMediumAutomaton_incomplete.rep_eq )
 
-lemma fairmediumautomaton_initialstate[simp]: "ndaInitialState\<cdot>fairMediumAutomaton = fairMediumInitials"
-  by(simp add: fairMediumAutomaton.rep_eq ndaInitialState.rep_eq)
+lemma fairmediumautomaton_initialstate[simp]: "ndaInitialState\<cdot>fairMediumAutomaton = (initCompletion chaosInit_h) fairMediumInitials"
+  apply(simp add: fairMediumAutomaton_def)
+  by(simp add: ndaInitialState.rep_eq fairMediumAutomaton_incomplete.rep_eq)
 
 lemma fairmediumautomaton_dom[simp]: "ndaDom\<cdot>fairMediumAutomaton = mediumDom"
-  by(simp add: fairMediumAutomaton.rep_eq ndaDom.rep_eq)
+  apply(simp add: fairMediumAutomaton_def)
+  by(simp add: ndaDom.rep_eq fairMediumAutomaton_incomplete.rep_eq)
 
 lemma fairmediumautomaton_ran[simp]: "ndaRan\<cdot>fairMediumAutomaton = mediumRan"
-  by(simp add: fairMediumAutomaton.rep_eq ndaRan.rep_eq)
+  apply(simp add: fairMediumAutomaton_def)
+  by(simp add: ndaRan.rep_eq fairMediumAutomaton_incomplete.rep_eq)
+
+
+section \<open>Consistent\<close>
+
+lemma fairmediumstep_consistent [simp]:  "uspecIsConsistent (fairMediumStep s)"
+  unfolding fairMediumStep_def
+  by(rule nda_consistent, simp_all)
+
+lemma fairmedium_consistent [simp]:  "uspecIsConsistent fairMediumSPS"
+  oops  (* ToDo *)
 
 
 section \<open>Step-wise lemmata for the transition function\<close>
 
 (* Line 15:  Single [counter!=0] / {counter=counter-1}; *)
-lemma fairMediumTransition_0_0:
+lemma fairMediumTransition_0_0[simp]:
   assumes "var_counter\<noteq>0"
     shows "fairMediumTransition ((FairMediumState Single var_counter), (mediumElemIn_i (Msg port_i)))
          = (Rev {(FairMediumState Single (var_counter-1), (mediumOut_o null))})"
   using assms by(auto simp add: fairMediumTransition_def assms)
 
 (* Line 16:  Single [counter==0] / {counter=rand{j. j>=0}, o=i}; *)
-lemma fairMediumTransition_0_1:
+lemma fairMediumTransition_0_1[simp]:
   assumes "var_counter=0"
     shows "fairMediumTransition ((FairMediumState Single var_counter), (mediumElemIn_i (Msg port_i)))
          = (Rev {(FairMediumState Single var_counter, (mediumOut_o (Msg (port_i)))) | var_counter . (var_counter>=0)})"
@@ -101,16 +122,22 @@ lemma fairMediumTransition_1_1:
 section \<open>Step-wise lemmata for the SPS\<close>
 
 (* Convert the SPS to step notation *)
-lemma fairMediumSps2Step: "fairMediumSPS = uspecFlatten mediumDom mediumRan
-    (Rev {spsConcOut (mediumOut_o null) (fairMediumStep (FairMediumState Single (var_counter::nat))) | var_counter . (var_counter>=0)})"
-  sorry
+lemma fairMediumSps2Step: "fairMediumSPS = ndaConcOutFlatten mediumDom mediumRan (initCompletion chaosInit_h fairMediumInitials) fairMediumStep"
+  by (simp add: fairMediumSPS_def fairMediumStep_def nda_H_def)
 
 (* Line 15:  Single [counter!=0] / {counter=counter-1}; *)
+
+(* SWS: So sollen erstmal alle steps aussehen. Die form klappt für alle *)
+(* Für die deterministischen steps kann man noch eine einfachere form generieren, ohne "ndaConcOutFlatten" *)
 lemma fairMediumStep_0_0:
   assumes "var_counter\<noteq>0"
     shows "spsConcIn  (mediumIn_i (Msg port_i)) (fairMediumStep (FairMediumState Single var_counter))
-         = spsConcOut (mediumOut_o null) (fairMediumStep (FairMediumState Single (var_counter-1)))"
-  oops
+         = ndaConcOutFlatten mediumDom mediumRan (initCompletion (Rev UNIV) (Rev {(FairMediumState Single (var_counter - 1), mediumOut_o -)})) fairMediumStep"
+  unfolding fairMediumStep_def mediumIn_i_def
+  apply(subst nda_h_I, simp_all)
+   apply (metis fairMediumStep_def fairmediumstep_consistent)
+  by(simp add: assms transCompletion_def chaosTrans_h_def)
+
 
 (* Line 16:  Single [counter==0] / {counter=rand{j. j>=0}, o=i}; *)
 lemma fairMediumStep_0_1:
